src/program_proof/examples/alloc_crash_proof.v
@@ -1,11 +1,11 @@
 From RecordUpdate Require Import RecordSet.
 From Perennial.Helpers Require Import Map gset.
 
-From Perennial.goose_lang Require Import crash_modality.
+From Perennial.goose_lang Require Import crash_modality crash_borrow.
 From Perennial.base_logic Require Import lib.ghost_map.
 
 From Goose.github_com.mit_pdos.perennial_examples Require Import alloc.
-From Perennial.program_logic Require Export na_crash_inv ncinv.
+From Perennial.program_logic Require Export ncinv.
 From Perennial.program_proof Require Import disk_prelude.
 From Perennial.program_proof.examples Require Import alloc_addrset.
 
